[WIP] Prove theorems in Nop.

coq/exec/Nop.v
@@ -58,23 +58,32 @@ Definition insert_nop (target:id) (bs:blocks): blocks :=
 Definition insert_nops (targets:list id) (bs:blocks): blocks :=
   List.fold_left (flip insert_nop) targets bs.
 
+Definition is_not_nop (c: cmd) :=
+  match c with
+    | insn_nop _ => false
+    |  _ => true
+  end.
+
+Definition nop_cmds (cmds_src cmds_tgt:cmds) :=
+  filter is_not_nop cmds_src = filter is_not_nop cmds_tgt.
+
 (* TODO: how about defining with filters? *)
-Inductive nop_cmds: forall (cmds_src cmds_tgt:cmds), Prop :=
-| nop_cmds_nil:
-    nop_cmds nil nil
-| nop_cmds_cons
-    c cmds_src cmds_tgt
-    (NOP: nop_cmds cmds_src cmds_tgt):
-    nop_cmds (c::cmds_src) (c::cmds_tgt)
-| nop_cmds_src
-    id cmds_src cmds_tgt
-    (NOP: nop_cmds cmds_src cmds_tgt):
-    nop_cmds ((insn_nop id)::cmds_src) cmds_tgt
-| nop_cmds_tgt
-    id cmds_src cmds_tgt
-    (NOP: nop_cmds cmds_src cmds_tgt):
-    nop_cmds cmds_src ((insn_nop id)::cmds_tgt)
-.
+(* Inductive nop_cmds: forall (cmds_src cmds_tgt:cmds), Prop := *)
+(* | nop_cmds_nil: *)
+(*     nop_cmds nil nil *)
+(* | nop_cmds_cons *)
+(*     c cmds_src cmds_tgt *)
+(*     (NOP: nop_cmds cmds_src cmds_tgt): *)
+(*     nop_cmds (c::cmds_src) (c::cmds_tgt) *)
+(* | nop_cmds_src *)
+(*     id cmds_src cmds_tgt *)
+(*     (NOP: nop_cmds cmds_src cmds_tgt): *)
+(*     nop_cmds ((insn_nop id)::cmds_src) cmds_tgt *)
+(* | nop_cmds_tgt *)
+(*     id cmds_src cmds_tgt *)
+(*     (NOP: nop_cmds cmds_src cmds_tgt): *)
+(*     nop_cmds cmds_src ((insn_nop id)::cmds_tgt) *)
+(* . *)
 
 Definition nop_blocks (blocks_src blocks_tgt:blocks): Prop :=
   forall bid,
@@ -91,28 +100,161 @@ Definition nop_blocks (blocks_src blocks_tgt:blocks): Prop :=
 Lemma lookupAL_mapAL A B i (f:A -> B) l:
   lookupAL _ (map f l) i = option_map f (lookupAL _ l i).
 Proof.
-Admitted.
+  induction l; simpl in *; auto.
+  destruct a.
+  destruct (i ==a); simpl; auto.
+Qed.
+
+Lemma filter_pop_tail : forall A f (l : list A) x,
+                          (filter f (l ++ [x])) =
+                          (filter f l) ++ (if (f x) then [x] else nil).
+Proof.
+  ii.
+  induction l0 as [|y l IH];
+    destruct (f x) eqn:T; simpl in *; auto; try (rewrite T; auto);
+    destruct (f y); simpl in *; try (rewrite <- IH; auto).
+Qed.
+
+Lemma nop_cmds_commutes : forall x y,
+                            nop_cmds x y -> nop_cmds y x.
+Proof.
+  unfold nop_cmds.
+  induction x; intros; simpl in *; auto.
+Qed.
+
+Lemma nop_blocks_commutes : forall x y,
+                            nop_blocks x y -> nop_blocks y x.
+Proof.
+  ii.
+  unfold nop_blocks.
+  unfold lift2_option.
+  destruct (lookupAL stmts y bid) eqn:T.
+  generalize dependent y.
+  induction x; intros; simpl in *; auto.
+  - unfold nop_blocks in H.
+    assert(G:=(H bid)).
+    simpl in G.
+    rewrite T in G.
+    inv G.
+  - destruct a;
+    destruct (bid == l0);
+    destruct s, s0;
+    destruct (lookupAL stmts x bid) eqn:T2;
+    subst; simpl.
+    +
+    unfold nop_blocks in H.
+    assert(G:= (H l0)).
+    rewrite T in G.
+    simpl in G.
+    Set Printing All.
+    unfold lift2_option in G.
+    Check (l0 == l0).
+    Admitted.
+    (* { *)
+    (*   assert(J: (if l0 == l0 *)
+    (*              then Some (stmts_intro phinodes0 cmds0 terminator0) *)
+    (*              else lookupAL stmts x l0) = Some (stmts_intro phinodes0 cmds0 terminator0)). *)
+    (*   destruct (l0 == l0); auto. unfold not in n. exploit n; auto. intro. inv x0. *)
+    (*   unfold lift2_option in G. *)
+    (*   simpl in G. *)
+    (* } *)
+
+
+
+(*     destruct *)
+(*       (if l0 == l0 *)
+(*          then Some (stmts_intro phinodes0 cmds0 terminator0) *)
+(*          else lookupAL stmts x l0) eqn:ABC. *)
+(*     cbn in ABC. *)
+(*     (* cbv in ABC. *) *)
+(*     hnf in ABC. *)
+
+(*     unfold lift2_option in G. *)
+(*     (* rewrite ABC in G. *) *)
+(*     destruct (l0 == l0) eqn:TT. *)
+(*     rewrite TT in G. *)
+(*     simpl in G. *)
+    
+(*     inv ABC. *)
+(*     destruct (l0 == l0) eqn:ABC. *)
+(*     inv H1. *)
+(*     Focus 2. admit. *)
+(*     cbv in H1. *)
+
+
+(*     rewrite J in G. *)
+(*     assert(J:= (eq_atom_dec l0 l0)). *)
+(*     destruct J. *)
+(*     Focus 2. unfold not in n. exploit n; auto. intro. inv x0. *)
+(*     splits.  *)
+(*     (* + destruct s. destruct s0. splits; auto. *) *)
+
+(*     admit. *)
+(*     admit. *)
+(*     (* destruct (lookupAL stmts x bid). *) *)
+(*     (* destruct s. destruct s1. splits. auto. *) *)
+(*   - destruct (lookupAL stmts x bid) eqn:T2. *)
+(*     admit. *)
+(*     auto. *)
+(* Admitted. *)
 
 Lemma insert_nop_spec1 id bs:
   nop_blocks bs (insert_nop id bs).
 Proof.
   ii. unfold insert_nop. rewrite lookupAL_mapAL.
-  destruct (lookupAL _ bs bid); simpl in *; auto.
-  destruct s; splits; auto.
+  unfold insert_at, nop_cmds.
+  destruct (lookupAL stmts bs bid) eqn:LOOKUP2; simpl in *; auto.
   repeat
     match goal with
-    | [|- context[match ?c with | Some _ => _ | None => _ end]] => destruct c
-    | [|- context[if ?c then _ else _]] => destruct c
-    end.
-  - admit.
-  - admit.
-  - admit.
-  - admit.
-Admitted.
+      | [|- context[match ?c with | Some _ => _ | None => _ end]] => destruct c
+      | [|- context[if ?c then _ else _]] => destruct c
+      | [|- context[let (_) := ?c in _]] => destruct c
+    end;
+    simpl; splits; auto.
+  - rewrite util.filter_app; simpl.
+  clear phinodes5 terminator5 LOOKUP2 bid id.
+  rewrite Nat.add_comm.
+  simpl.
+  rewrite <- util.filter_app.
+  rewrite firstn_skipn.
+  auto.
+  - rewrite util.filter_app.
+  simpl. rewrite <- util.filter_app.
+  rewrite firstn_skipn. auto.
+Qed.
 
+Lemma gggg : forall n m,
+               (fix mul (n0 m0 : nat) {struct n0} : nat :=
+                  match n0 with
+                    | 0%nat => 0%nat
+                    | S p => (m0 + mul p m0)%nat
+                  end) n m
+               =
+               match n with
+                 | 0%nat => 0%nat
+                 | S p => (m +
+                           (fix mul (n0 m0 : nat) {struct n0} : nat :=
+                  match n0 with
+                    | 0%nat => 0%nat
+                    | S p => (m0 + mul p m0)%nat
+                  end) p m)%nat
+               end
+.
+Proof.
+  induction n; intros; auto.
+Qed.
+(* Lemma ggg : forall n m, Nat.mul n m = 0%nat. *)
+(* Proof. *)
+(*   intros. *)
+(*   unfold Nat.mul. *)
+(*   simpl. *)
+(* Qed. *)
 Lemma insert_nop_spec2 id bs:
   nop_blocks (insert_nop id bs) bs.
 Proof.
+  apply nop_blocks_commutes.
+  apply insert_nop_spec1.
+Qed.
   ii. unfold insert_nop. rewrite lookupAL_mapAL.
   destruct (lookupAL _ bs bid); simpl in *; auto.
   destruct s; splits; auto.
